AllStar/SubparserTests.v
@@ -1,8 +1,9 @@
 Require Import List String.
-Require Import ExampleGrammars Grammar Subparser.
+Require Import ExampleGrammars Grammar Subparser Lib.Utils.
 Import ListNotations.
+Require Import Grammar.
 
-Print g312.
+(* Grammar 3.12 *)
 (*
 [(NT "Z", [T "d"]); 
  (NT "Z", [NT "X"; NT "Y"; NT "Z"]); 
@@ -10,23 +11,59 @@ Print g312.
  (NT "Y", [T "c"]); 
  (NT "X", [NT "Y"]); 
  (NT "X", [T "a"])]
-*)
+ *)
+
+(* spClosure works with an empty stack *)
+Example spClosureTest1 :
+  spClosure g312 (nonterminals g312) {| stack := nil; pred := [T "d"] |} =
+  [{| stack := nil; pred := [T "d"] |}].
+Proof.
+  unfold spClosure. simpl. reflexivity.
+Qed.
+
+(* it also works when the top stack element is a terminal *)
+Example spClosureTest2 :
+  spClosure g312 (nonterminals g312) {| stack := [T "d"]; pred := [T "d"] |} =
+  [{| stack := [T "d"]; pred := [T "d"] |}].
+Proof.
+  unfold spClosure. simpl. reflexivity.
+Qed.
+
+Example spClosureTest3 :
+  spClosure g312 (nonterminals g312) {| stack := [NT "out-of-vocab"]; pred := [T "d"] |} = nil.
+Proof.
+  unfold spClosure. simpl. reflexivity.
+Qed.
+
+Example spClosureTest4 :
+  spClosure g312
+            (nonterminals g312)
+            {| stack := [NT "X"; NT "Y"; NT "Z"];
+               pred := [NT "X"; NT "Y"; NT "Z"] |} =
+  [{|
+      stack := [T "c"; NT "Y"; NT "Z"];
+      pred := [NT "X"; NT "Y"; NT "Z"]
+   |};
+   {|
+     stack := [T "a"; NT "Y"; NT "Z"];
+     pred := [NT "X"; NT "Y"; NT "Z"]
+   |}].
+Proof. compute. reflexivity. Qed.
 
 Example Z_abc : 
   adaptivePredict g312 "Z" ["a"; "b"; "c"] nil =
   Choice [NT "X"; NT "Y"; NT "Z"].
-Proof. compute. Abort.
+Proof. compute. reflexivity. Qed. 
 
 Example Z_ababd :
   adaptivePredict g312 "Z" ["a"; "b"; "a"; "b"; "d"] nil = 
   Choice [NT "X"; NT "Y"; NT "Z"].
-Proof. compute. Abort.
+Proof. compute. reflexivity. Qed.
 
 Example X_a : 
   exists sps, adaptivePredict g312 "X" ["a"] nil =
               Conflict sps.
-Proof. 
-  eexists. compute. Abort.
+Proof. eexists. compute. reflexivity. Qed.
 
 (* Should this really be an unambiguous choice, 
    or should we report a conflict,
